"recursive function will be detected. but there's termination proof problem"

smtlink/z3_files/test5.py
@@ -1,0 +1,8 @@
+from sys import path
+path.insert(0,"/ubc/cs/home/y/yanpeng/project/ACL2/smtlink/z3_interface")
+from ACL2_translator import to_smt, Q
+s = to_smt()
+A=s.isReal("A")
+hypothesis=s.notx(s.lt(A,10))
+conclusion=s.notx(s.lt((lambda var0:s.ifx(False,1,s.times(var0,False)))(A),20))
+s.prove(hypothesis, conclusion)
