smtlink/helper.lisp
@@ -1,6 +1,22 @@
 ;; helper functions for basic data structure manipulation
 (in-package "ACL2")
 
+;; exist
+(defun exist (elem lista)
+  "exist: check if an element exist in a list"
+  (if (endp lista)
+      nil
+    (if (equal elem (car lista))
+	t
+      (exist elem (cdr lista)))))
+
+;; end
+(defun end (lista)
+  "end: return the last element in a list"
+  (if (endp (cdr lista))
+      (car lista)
+    (end (cdr lista))))
+
 ;; my-last
 (defun my-last (listx)
  "my-last: fetch the last element from list"
@@ -15,3 +31,7 @@
 	  (cdr listx)
 	  (cons (car listx)
 		(my-delete (cdr listx) elem)))))
+
+(defthm delete-must-reduce
+    (implies (exist a listx)
+	     (< (len (my-delete listx a)) (len listx))))
